src/Locking.v
@@ -1,0 +1,59 @@
+Require Import EventCSL.
+Require Import Hlist.
+
+Set Implicit Arguments.
+
+Section Locking.
+
+Variable Mcontents : list Set.
+Variable Scontents : list Set.
+
+Notation S := (hlist (fun T:Set => T) Scontents).
+
+Inductive MutexOwner : Set :=
+| NoOwner
+| Owned (id:ID).
+
+(** given a lock variable and some other variable v, generate a
+relation for tid that makes the variable read-only for non-owners. *)
+Definition lock_protects (lvar : var Scontents MutexOwner)
+           {tv} (v : var Scontents tv) tid (s s': S) :=
+  forall owner_tid,
+    get lvar s = Owned owner_tid ->
+    tid <> owner_tid ->
+    get v s' = get v s.
+
+Hint Unfold lock_protects : prog.
+
+Inductive lock_protocol (lvar : var Scontents MutexOwner) (tid : ID) : S -> S -> Prop :=
+| NoChange : forall s s', get lvar s  = get lvar s' ->
+                     lock_protocol lvar tid s s'
+| OwnerRelease : forall s s', get lvar s = Owned tid ->
+                         get lvar s' = NoOwner ->
+                         lock_protocol lvar tid s s'
+| OwnerAcquire : forall s s', get lvar s = NoOwner ->
+                         get lvar s' = Owned tid ->
+                         lock_protocol lvar tid s s'.
+
+Hint Constructors lock_protocol.
+
+Inductive ghost_lock_invariant
+          (lvar : var Mcontents Mutex)
+          (glvar : var Scontents MutexOwner)
+          (m : M Mcontents) (s : S) : Prop :=
+| LockOpen : get lvar m = Open -> get glvar s = NoOwner ->
+             ghost_lock_invariant lvar glvar m s
+| LockOwned : forall tid, get lvar m = Locked -> get glvar s = Owned tid ->
+                     ghost_lock_invariant lvar glvar m s.
+
+Hint Constructors ghost_lock_invariant.
+
+Lemma ghost_lock_owned : forall lvar glvar m s tid,
+    ghost_lock_invariant lvar glvar m s ->
+    get glvar s = Owned tid ->
+    get lvar m = Locked.
+Proof.
+  inversion 1; congruence.
+Qed.
+
+End Locking.
